finish fomega preservation

Fomega/Basic/Preservation.lean
@@ -19,14 +19,17 @@ namespace Fomega.Proof
 
   theorem lam_destruct_lemma : Judgment v Γ ix -> LamDestructLemmaType Γ v ix := by
   intro j; induction j <;> simp at *
-  case lam A' _ _ B' _ j1 j2 j3 ih1 ih2 ih3 => sorry
-    -- intro m C A b B h1 h2 h3 x r1 r2
-    -- apply And.intro; subst h1; rfl; subst h1; subst h2; subst h3
-    -- have lem := @RedConv.all_congr _ A' B' _ A B (by exists x)
-    -- apply And.intro; apply RedConv.sym; apply lem.2.1
-    -- exists B'; apply And.intro; apply RedConv.sym; apply lem.2.2
-    -- apply j3
-  case conv A' B' _ _ _ cv ih1 _ih2 => sorry
+  case lam A' K1 K2 B' t j1 j2 j3 _ _ _ =>
+    intro m C A b B h1 h2 h3 x r1 r2; subst h1; subst h2; subst h3
+    have lem := @RedConv.all_congr _ A B _ A' B' (by exists x)
+    simp; apply And.intro; apply And.intro; apply lem.2.1
+    exists (dom K1 K2); exists K2; exists B'; apply And.intro
+    apply lem.2.2; apply And.intro; apply j2; apply j3
+  case conv A' B' _ _ _ cv ih1 _ih2 =>
+    intro m C A b B h1 x r1 r2; cases cv; case _ w r3 =>
+      have lem := Red.confluence r1 r3.2
+      cases lem; case _ q r4 =>
+        apply ih1 m C A b B h1 q (Red.trans r3.1 r4.2) (Red.trans r2 r4.1)
 
   inductive CtxRed : Ctx -> Ctx -> Prop where
   | nil : CtxRed [] []
@@ -34,7 +37,6 @@ namespace Fomega.Proof
   | tail : CtxRed Γ Γ' -> CtxRed (A::Γ) (A::Γ')
 
   namespace CtxRed
-
     theorem refl : CtxRed Γ Γ := by
     induction Γ
     case _ => constructor
@@ -55,15 +57,18 @@ namespace Fomega.Proof
         cases (ih x)
         case _ h => apply Or.inl; rw [h]
         case _ h => apply Or.inr; apply Red.subst1_same; apply h
-
   end CtxRed
 
+  inductive CtxRedStar : Ctx -> Ctx -> Prop where
+  | refl : CtxRedStar t t
+  | step : CtxRed x y -> CtxRedStar y z -> CtxRedStar x z
+
   @[simp]
-  abbrev PreservationType (Γ : Ctx) : (v : JudgmentVariant) -> JudgmentIndex v -> Prop
+  abbrev Preservation1Type (Γ : Ctx) : (v : JudgmentVariant) -> JudgmentIndex v -> Prop
   | .prf => λ (t, A) => ∀ {t' Γ'}, t = t' ∨ t -β> t' -> CtxRed Γ Γ' -> Γ' ⊢ t' : A
   | .wf => λ () => ∀ {Γ'}, CtxRed Γ Γ' -> ⊢ Γ'
 
-  theorem preservation1 : Judgment v Γ ix -> PreservationType Γ v ix := by
+  theorem preservation1 : Judgment v Γ ix -> Preservation1Type Γ v ix := by
   intro j; induction j <;> simp at *
   case nil =>
     intro Γ' r
@@ -92,7 +97,20 @@ namespace Fomega.Proof
         exists (Γ' d@ x); apply And.intro
         apply RedStar.refl; apply Red.trans_flip RedStar.refl h2
     case _ r1 => cases r1
-  case pi => sorry
+  case pi Γ A K1 K2 B j1 j2 ih1 ih2 =>
+    intro t' Γ' r1 r2
+    cases r1
+    case _ r1 =>
+      rw [<-r1]; constructor; apply ih1 (Or.inl rfl) r2
+      apply ih2 (Or.inl rfl) (.tail r2)
+    case _ r1 =>
+      cases r1
+      case _ A' r1 =>
+        constructor; apply ih1 (Or.inr r1) r2
+        apply ih2 (Or.inl rfl) (.head r1 r2)
+      case _ B' r1 =>
+        constructor; apply ih1 (Or.inl rfl) r2
+        apply ih2 (Or.inr r1) (.tail r2)
   case lam Γ A K1 K2 B t j1 j2 j3 ih1 ih2 ih3 =>
     intro t' Γ' r1 r2
     cases r1
@@ -174,142 +192,52 @@ namespace Fomega.Proof
     constructor; apply ih1 r1 r2; apply ih2 (Or.inl rfl) r2
     apply j3
 
-  -- abbrev ctx_red x Γ Γ' := ∀ n, Γ d@ x -β> Γ' d@ x ∧ (n ≠ x -> Γ d@ n = Γ' d@ n)
+  theorem preservation_term : Γ ⊢ t : A -> t -β>* t' -> Γ ⊢ t' : A := by
+  intro j r; induction r
+  case _ => apply j
+  case _ r1 _r2 ih =>
+    have lem := preservation1 j (Or.inr r1) CtxRed.refl
+    apply ih lem
 
-  -- theorem ctx_red_lift : ctx_red x Γ Γ' -> ctx_red (x + 1) (A::Γ) (A::Γ') := by sorry
+  theorem preservation_ctx : Γ ⊢ t : A -> CtxRedStar Γ Γ' -> Γ' ⊢ t : A := by
+  intro j r; induction r
+  case _ => apply j
+  case _ r1 _r2 ih =>
+    have lem := preservation1 j (Or.inl rfl) r1
+    apply ih lem
 
-  -- theorem preservation_ctx_lift : (∀ n, Γ d@ n -β> Δ d@ n ∨ Γ d@n = Δ d@ n) ->
-  --   A -β> A' ∨ A = A' ->
-  --   ∀ n, (A::Γ) d@ n -β> (A'::Δ) d@ n ∨ (A::Γ) d@n = (A'::Δ) d@ n
-  -- := by sorry
+  theorem preservation_type : Γ ⊢ t : A -> A -β>* A' -> Γ ⊢ t : A' := by
+  intro j r
+  have lem := classification j
+  cases lem
+  case _ h =>
+    subst h; cases r; apply j
+    case _ r _ => cases r
+  case _ h =>
+    cases h; case _ K h =>
+      apply Judgment.conv; apply j
+      apply preservation_term; apply h; apply r
+      exists A'; apply And.intro; apply r; apply Red.refl
 
-  -- theorem preservation1_term : Γ ⊢ t : A ->
-  --   (∀ n, Γ d@ n -β> Δ d@ n ∨ Γ d@n = Δ d@ n) ->
-  --   Δ ⊢ t : A ∧ (∀ t', t -β> t' -> Δ ⊢ t' : A)
-  -- := by
-  -- intro j h
-  -- induction j generalizing Δ
-  -- case ax Γ f j ih =>
-  --   apply And.intro
-  --   case _ =>
-  --     apply Proof.ax f
-  --     intro x
-  --     cases (h x)
-  --     case _ hx => apply (ih x h).2 _ hx
-  --     case _ hx => rw [<-hx]; apply (ih x h).1
-  --   case _ => intro t' r; cases r
-  -- case var Γ x K j ih =>
-  --   apply And.intro
-  --   case _ =>
-  --     constructor; constructor
-  --     cases (h x)
-  --     case _ hx => apply (ih h).2 _ hx
-  --     case _ hx => rw [<-hx]; apply (ih h).1
-  --     apply (ih h).1
-  --     cases (h x)
-  --     case _ hx =>
-  --       exists (Δ d@ x); apply And.intro
-  --       apply Term.Red.refl; apply Term.RedStar.step; apply hx; apply Term.Red.refl
-  --     case _ hx => rw [hx]; apply Term.RedConv.refl
-  --   case _ => intro t' r; cases r
-  -- case pi Γ A K B j1 j2 ih1 ih2 =>
-  --   apply And.intro
-  --   case _ =>
-  --     constructor
-  --     apply (ih1 h).1
-  --     apply (@ih2 (A::Δ) (preservation_ctx_lift h (Or.inr rfl))).1
-  --   case _ => sorry
-  -- case tpi => sorry
-  -- case lam Γ A B K t j1 j2 ih1 ih2 =>
-  --   apply And.intro
-  --   case _ =>
-  --     constructor
-  --     apply (ih1 h).1
-  --     apply (@ih2 (A::Δ) (preservation_ctx_lift h (Or.inr rfl))).1
-  --   case _ =>
-  --     intro t' r
-  --     cases r
-  --     case lam_congr1 A' r =>
-  --       constructor; constructor
-  --       apply (ih1 h).2 _ (Term.Red.all_congr1 r)
-  --       apply (@ih2 (A'::Δ) (preservation_ctx_lift h (Or.inl r))).1
-  --       apply (ih1 h).1
-  --       exists (.all mf A' B); apply And.intro
-  --       apply Term.Red.refl
-  --       apply Term.Red.congr1 (λ A => .all mf A B) Term.Red.all_congr1
-  --       apply Term.RedStar.step r; apply Term.Red.refl
-  --     case lam_congr2 t' r =>
-  --       constructor; apply (ih1 h).1
-  --       apply (@ih2 (A::Δ) (preservation_ctx_lift h (Or.inr rfl))).2 _ r
-  -- case app Γ f A B a B' j1 j2 j3 ih1 ih2 =>
-  --   apply And.intro
-  --   case _ =>
-  --     constructor
-  --     apply (ih1 h).1; apply (ih2 h).1; apply j3
-  --   case _ =>
-  --     intro t' r
-  --     sorry
-  -- case econv Γ t A B K j1 j2 j3 ih1 ih2 =>
-  --   apply And.intro
-  --   case _ =>
-  --     constructor
-  --     apply (ih1 h).1; apply (ih2 h).1; apply j3
-  --   case _ =>
-  --     intro t' r
-  --     sorry
-  -- case iconv Γ t A B K j1 j2 j3 ih1 ih2 =>
-  --   apply And.intro
-  --   case _ =>
-  --     constructor
-  --     apply (ih1 h).1; apply (ih2 h).1; apply j3
-  --   case _ => sorry
+  theorem preservation_wf : ⊢ Γ -> CtxRedStar Γ Γ' -> ⊢ Γ' := by
+  intro j r
+  induction r
+  case _ => apply j
+  case _ r1 _r2 ih =>
+    have lem := preservation1 j r1
+    apply ih lem
 
-  -- theorem preservation_jud : Γ ⊢ t : A ->
-  --   (∀ t', t -β> t' -> Γ ⊢ t' : A)
-  --   ∧ (∀ x Γ', ctx_red x Γ Γ' -> Γ' ⊢ t : A)
-  --   ∧ (∀ x Γ', ctx_red x Γ Γ' -> t = Γ d@ x -> Γ' ⊢ Γ' d@ x : A)
-  -- := by
-  -- intro j
-  -- induction j
-  -- case ax Γ f h ih =>
-  --   apply And.intro
-  --   intro t' r; cases r
-  --   sorry
-  -- case var Γ i K h ih =>
-  --   have ih1 := ih.1; have ih2 := ih.2.1; have ih3 := ih.2.2; clear ih
-  --   apply And.intro
-  --   case _ => intro t' r; cases r
-  --   apply And.intro
-  --   case _ =>
-  --     intro x Γ' r
-  --     cases Nat.decEq i x
-  --     case _ hv =>
-  --       rw [(r i).2 hv] at *; constructor
-  --       apply ih2 _ _ r
-  --     case _ hv =>
-  --       subst hv
-  --       constructor; constructor
-  --       apply ih3 i _ r; rfl
-  --       apply ih2 _ _ r
-  --       exists (Γ' d@ i); apply And.intro; apply Term.RedStar.refl
-  --       apply Term.RedStar.step; apply (r i).1; apply Term.RedStar.refl
-  --   case _ =>
-  --     intro x Γ' r ht
-  --     replace r := (r x).1; rw [<-ht] at r
-  --     cases r
-  -- case pi => sorry
-  -- case tpi => sorry
-  -- case lam => sorry
-  -- case app => sorry
-  -- case econv => sorry
-  -- case iconv => sorry
-
-  -- theorem preservation : Γ ⊢ t : A -> t -β>* t' -> Γ ⊢ t' : A := by
-  -- intro j r
-  -- induction r generalizing Γ A
-  -- case _ => exact j
-  -- case _ r1 _r2 ih => apply ih (preservation1 j r1)
-
-  theorem preservation_type : Γ ⊢ t : A -> A -β>* A' -> Γ ⊢ t : A' := by sorry
+  theorem preservation :
+    Γ ⊢ t : A ->
+    CtxRedStar Γ Γ' ->
+    t -β>* t' ->
+    A -β>* A' ->
+    Γ' ⊢ t' : A'
+  := by
+  intro j r1 r2 r3
+  replace j := preservation_ctx j r1
+  replace j := preservation_term j r2
+  replace j := preservation_type j r3
+  apply j
 
 end Fomega.Proof
